Recovered all examples except verif_mark_bi_dag.

sample_mark/unionfind_arr.c
@@ -21,7 +21,7 @@ int find(struct subset subsets[], int i)
     }
  
     return p;
-}
+} 
 
 void Union(struct subset subsets[], int x, int y)
 {
